

$$\text{Var } X = \frac{1}{N} \sum_{n=0}^N (x_n - \bar{x}_n)^2$$

Let  $S_n = N \cdot \text{Var } X$ .  $S_n$  can be expressed,

$$S_n = S_{n-1} + (x_n - \mu_{n-1})(x_n - \mu_n).$$

This equality can be proven by,

$$\begin{aligned} S_n &= N \cdot \text{Var } X \\ &= N \cdot \frac{1}{N} \sum_{i=0}^N (x_i - \bar{x}_n)^2 \\ &= \sum_{i=0}^n (x_i^2 - 2\bar{x}_n x_i + \bar{x}_n^2) \\ &= \sum_{i=0}^n x_i^2 - 2\bar{x}_n \sum_{i=0}^n x_i + \bar{x}_n^2 \sum_{i=0}^n 1 \\ &= \sum x_i^2 - 2\bar{x}_n n \frac{\sum x_i}{n} + n \bar{x}_n^2 \\ &= \sum x_i^2 - 2\bar{x}_n^2 n + n \bar{x}_n^2 \\ &= \sum x_i^2 + n \bar{x}_n^2 (-2 + 1) \\ &= \sum x_i^2 - n \bar{x}_n^2 \end{aligned}$$

This expression can be used to express  $S_{n-1}$ .

$$S_{n-1} = \sum_{i=0}^{n-1} x_i^2 - (n-1) \bar{x}_{n-1}^2$$

The incremental difference between  $S_n$  and  $S_{n-1}$  can be found by converting the closed form of the series into a recurrence relation.

$$S_n - S_{n-1} = \sum x_i^2 - n \bar{x}_n^2 - \left[ \sum_{i=0}^{n-1} x_i^2 - (n-1) \bar{x}_{n-1}^2 \right]$$

$$\begin{aligned}
&= \sum_{i=1}^n x_i^2 - \sum_{i=1}^{n-1} x_i^2 - n\bar{x}_n^2 + (n-1)\bar{x}_{n-1}^2 \\
&= x_n^2 - n\bar{x}_n^2 + n\bar{x}_{n-1}^2 - \bar{x}_{n-1}^2 \\
&= x_n^2 + n(\bar{x}_{n-1}^2 - \bar{x}_n^2) - \bar{x}_{n-1}^2 \\
&= x_n^2 + n(\bar{x}_{n-1} + \bar{x}_n)(\bar{x}_{n-1} - \bar{x}_n) - \bar{x}_{n-1}^2
\end{aligned}$$

Given the identity,

$$\begin{aligned}
x_n &= n\bar{x}_n - (n-1)\bar{x}_{n-1} \\
&= n(\bar{x}_n - \bar{x}_{n-1}) + \bar{x}_{n-1}
\end{aligned}$$

$$\bar{x}_{n-1} - x_n = n(\bar{x}_n - \bar{x}_{n-1})(-1)$$

$$\bar{x}_{n-1} - x_n = n(\bar{x}_{n-1} - \bar{x}_n) \quad \text{• producing the factor } \bar{x}_{n-1} - \bar{x}_n.$$

$$\bar{x}_{n-1} - \bar{x}_n = \frac{\bar{x}_{n-1} - x_n}{n} \quad \text{• isolating } \bar{x}_{n-1} - \bar{x}_n.$$

Sub in the equivalent expression and reduce the expression,

$$\begin{aligned}
&= x_n^2 + n(\bar{x}_{n-1} + \bar{x}_n)(\bar{x}_{n-1} - \bar{x}_n) - \bar{x}_{n-1}^2 \\
&= x_n^2 + n(\bar{x}_{n-1} + \bar{x}_n) \frac{(\bar{x}_{n-1} - x_n)}{n} - \bar{x}_{n-1}^2 \\
&= x_n^2 + (\bar{x}_{n-1} + \bar{x}_n)(\bar{x}_{n-1} - x_n) - \bar{x}_{n-1}^2 \\
&= x_n^2 + \bar{x}_{n-1}^2 - x_n \bar{x}_{n-1} + \bar{x}_n \bar{x}_{n-1} - \bar{x}_n x_n - \bar{x}_{n-1}^2 \\
&= x_n^2 - x_n \bar{x}_{n-1} + \bar{x}_n \bar{x}_{n-1} - \bar{x}_n x_n \\
&= (x_n - \bar{x}_{n-1})(x_n - \bar{x}_n) \\
&= S_n - S_{n-1}
\end{aligned}$$

Thus,

$$S_n = S_{n-1} + (x_n - \bar{x}_{n-1})(x_n - \bar{x}_n)$$

This implies,

$$\text{Var}_n(x) = \frac{n-1}{n} \text{Var}_{n-1}x + \frac{1}{n} (x_n - \bar{x}_{n-1})(x_n - \bar{x}_n)$$